<?xml version="1.0"?>
<rdf:RDF xmlns="http://www.essepuntato.it/2015/07/ido/"
     xml:base="http://www.essepuntato.it/2015/07/ido/"
     xmlns:schema="http://schema.org/"
     xmlns:owl="http://www.w3.org/2002/07/owl#"
     xmlns:xsd="http://www.w3.org/2001/XMLSchema#"
     xmlns:skos="http://www.w3.org/2004/02/skos/core#"
     xmlns:rdfs="http://www.w3.org/2000/01/rdf-schema#"
     xmlns:gr="http://purl.org/goodrelations/v1#"
     xmlns:frbr="http://purl.org/vocab/frbr/core#"
     xmlns:skos1="http://www.w3.org/2008/05/skos#"
     xmlns:rdf="http://www.w3.org/1999/02/22-rdf-syntax-ns#"
     xmlns:terms="http://purl.org/dc/terms/"
     xmlns:ti="http://www.ontologydesignpatterns.org/cp/owl/timeinterval.owl#"
     xmlns:xml="http://www.w3.org/XML/1998/namespace"
     xmlns:foaf="http://xmlns.com/foaf/0.1/"
     xmlns:dc="http://purl.org/dc/elements/1.1/"
     xmlns:sioc="http://rdfs.org/sioc/ns#">
    <owl:Ontology rdf:about="http://www.essepuntato.it/2015/07/ido-orders">
        <owl:versionIRI rdf:resource="http://www.essepuntato.it/2015/07/ido-orders/1.0"/>
        <owl:imports rdf:resource="http://www.essepuntato.it/2015/07/ido-items/1.0"/>
        <owl:imports rdf:resource="http://www.essepuntato.it/2015/07/ido-prices/1.0"/>
        <dc:rights xml:lang="it">Questo lavoro è distribuito sotto una licenza [Creative Commons Attribution 4.0 International (CC BY 4.0)](http://creativecommons.org/licenses/by/4.0/).</dc:rights>
        <rdfs:comment xml:lang="it">L&apos;Ontologia per i dati di Imperial (o Imperial Data Ontology, IDO) è un&apos;ontologia OWL 2 DL creata per la descrizione dei dati di vendita di aziende di moda. Questo modulo si preoccupa della descrizione degli ordini e delle fatture.</rdfs:comment>
        <dc:description rdf:resource="http://www.essepuntato.it/2015/07/ido/ido-orders.png"/>
        <owl:versionInfo rdf:datatype="http://www.w3.org/2001/XMLSchema#decimal">1.0</owl:versionInfo>
        <rdfs:comment xml:lang="en">The Imperial Data Ontology (IDO) is an OWL 2 DL ontology that allows the description of selling data of fashion design industries. This module describes the orders and the invoices.</rdfs:comment>
        <dc:title xml:lang="it">Ontologia per i dati di Imperial (IDO): modulo &quot;Ordini&quot;</dc:title>
        <dc:title xml:lang="en">Imperial Data Ontology (IDO): module &quot;Orders&quot;</dc:title>
        <dc:creator>Silvio Peroni (http://orcid.org/0000-0003-0530-4305)</dc:creator>
        <dc:date>2016-04-08</dc:date>
        <rdfs:label>IDO-O</rdfs:label>
        <dc:rights xml:lang="en">This work is distributed under a [Creative Commons Attribution 4.0 International (CC BY 4.0)](http://creativecommons.org/licenses/by/4.0/).</dc:rights>
    </owl:Ontology>
    


    <!-- 
    ///////////////////////////////////////////////////////////////////////////////////////
    //
    // Annotation properties
    //
    ///////////////////////////////////////////////////////////////////////////////////////
     -->

    


    <!-- http://www.w3.org/2000/01/rdf-schema#isDefinedBy -->

    <owl:AnnotationProperty rdf:about="http://www.w3.org/2000/01/rdf-schema#isDefinedBy"/>
    


    <!-- http://www.w3.org/2002/07/owl#cardinality -->

    <owl:AnnotationProperty rdf:about="http://www.w3.org/2002/07/owl#cardinality"/>
    


    <!-- 
    ///////////////////////////////////////////////////////////////////////////////////////
    //
    // Datatypes
    //
    ///////////////////////////////////////////////////////////////////////////////////////
     -->

    


    <!-- http://www.w3.org/2001/XMLSchema#date -->

    <rdfs:Datatype rdf:about="http://www.w3.org/2001/XMLSchema#date"/>
    


    <!-- http://www.w3.org/2001/XMLSchema#dateTime -->

    <rdfs:Datatype rdf:about="http://www.w3.org/2001/XMLSchema#dateTime"/>
    


    <!-- http://www.w3.org/2001/XMLSchema#float -->

    <rdfs:Datatype rdf:about="http://www.w3.org/2001/XMLSchema#float"/>
    


    <!-- 
    ///////////////////////////////////////////////////////////////////////////////////////
    //
    // Object Properties
    //
    ///////////////////////////////////////////////////////////////////////////////////////
     -->

    


    <!-- http://purl.org/goodrelations/v1#typeOfGood -->

    <owl:ObjectProperty rdf:about="http://purl.org/goodrelations/v1#typeOfGood">
        <rdfs:domain rdf:resource="http://purl.org/goodrelations/v1#TypeAndQuantityNode"/>
        <rdfs:range>
            <owl:Class>
                <owl:unionOf rdf:parseType="Collection">
                    <rdf:Description rdf:about="http://purl.org/goodrelations/v1#Individual"/>
                    <rdf:Description rdf:about="http://purl.org/goodrelations/v1#SomeItems"/>
                </owl:unionOf>
            </owl:Class>
        </rdfs:range>
        <rdfs:comment xml:lang="it">Questa proprietà permette di specificare un certo pezzo o una sua tipologia (cioè, un articolo gestito in magazzino) come indicato in un ordine o in una fattura.</rdfs:comment>
        <rdfs:comment xml:lang="en">This property allows one to specify a particular piece or its kind (i.e., a stock keeping unit) as listed either in an order or in an invoice.</rdfs:comment>
        <rdfs:isDefinedBy rdf:resource="http://purl.org/goodrelations/v1"/>
        <rdfs:label xml:lang="it">ha tipo di bene</rdfs:label>
        <rdfs:label xml:lang="en">has type of good</rdfs:label>
    </owl:ObjectProperty>
    


    <!-- http://schema.org/orderedItem -->

    <owl:ObjectProperty rdf:about="http://schema.org/orderedItem">
        <rdfs:domain>
            <owl:Class>
                <owl:unionOf rdf:parseType="Collection">
                    <rdf:Description rdf:about="http://schema.org/Order"/>
                    <rdf:Description rdf:about="http://schema.org/OrderItem"/>
                </owl:unionOf>
            </owl:Class>
        </rdfs:domain>
        <rdfs:range>
            <owl:Class>
                <owl:unionOf rdf:parseType="Collection">
                    <rdf:Description rdf:about="http://schema.org/OrderItem"/>
                    <rdf:Description rdf:about="http://schema.org/Product"/>
                </owl:unionOf>
            </owl:Class>
        </rdfs:range>
        <rdfs:comment xml:lang="it">La relazione che mette in relazione un ordine con la quantità di capi da esso descritti.</rdfs:comment>
        <rdfs:comment xml:lang="en">The link between an order and the amount of items which it includes.</rdfs:comment>
        <rdfs:isDefinedBy rdf:resource="http://schema.org"/>
        <rdfs:label xml:lang="it">include come articolo ordinato</rdfs:label>
        <rdfs:label xml:lang="en">includes as ordered article</rdfs:label>
    </owl:ObjectProperty>
    


    <!-- http://schema.org/partOfInvoice -->

    <owl:ObjectProperty rdf:about="http://schema.org/partOfInvoice">
        <owl:inverseOf rdf:resource="http://schema.org/referencesOrder"/>
        <rdfs:comment xml:lang="en">It allows one to specify that the order in consideration is being paid as part of the referenced invoice.</rdfs:comment>
        <rdfs:comment xml:lang="it">Permette di specificare che l&apos;ordine in considerazione è stato pagato come parte della ricevuta a cui si riferisce.</rdfs:comment>
        <rdfs:isDefinedBy rdf:resource="http://schema.org"/>
        <rdfs:label xml:lang="en">is part of invoice</rdfs:label>
        <rdfs:label xml:lang="it">è parte della ricevuta</rdfs:label>
    </owl:ObjectProperty>
    


    <!-- http://schema.org/referencesOrder -->

    <owl:ObjectProperty rdf:about="http://schema.org/referencesOrder">
        <rdfs:domain rdf:resource="http://schema.org/Invoice"/>
        <rdfs:range rdf:resource="http://schema.org/Order"/>
        <rdfs:comment xml:lang="en">It allows one to specify the order associated to the invoice in consideration.</rdfs:comment>
        <rdfs:comment xml:lang="it">Permette di specificare l&apos;ordine associato alla ricevuta in considerazione.</rdfs:comment>
        <rdfs:isDefinedBy rdf:resource="http://schema.org"/>
        <rdfs:label xml:lang="en">references order</rdfs:label>
        <rdfs:label xml:lang="it">si riferisce all&apos;ordine</rdfs:label>
    </owl:ObjectProperty>
    


    <!-- http://schema.org/totalPaymentDue -->

    <owl:ObjectProperty rdf:about="http://schema.org/totalPaymentDue">
        <rdfs:domain rdf:resource="http://schema.org/Invoice"/>
        <rdfs:range rdf:resource="http://schema.org/PriceSpecification"/>
        <rdfs:comment xml:lang="en">It allows to specify the total amount paid related to an invoice.</rdfs:comment>
        <rdfs:comment xml:lang="it">Permette di specificare la somma totale pagata in riferimento ad una ricevuta.</rdfs:comment>
        <rdfs:isDefinedBy rdf:resource="http://schema.org"/>
        <rdfs:label xml:lang="it">ha somma totale da pagare</rdfs:label>
        <rdfs:label xml:lang="en">has total payment due</rdfs:label>
    </owl:ObjectProperty>
    


    <!-- http://www.essepuntato.it/2015/07/ido/hasPricePerPiece -->

    <owl:ObjectProperty rdf:about="http://www.essepuntato.it/2015/07/ido/hasPricePerPiece">
        <rdfs:domain>
            <owl:Class>
                <owl:unionOf rdf:parseType="Collection">
                    <rdf:Description rdf:about="http://www.essepuntato.it/2015/07/ido/PieceWithPrice"/>
                    <rdf:Description rdf:about="http://www.essepuntato.it/2015/07/ido/StockKeepingUnitAmount"/>
                </owl:unionOf>
            </owl:Class>
        </rdfs:domain>
        <rdfs:range rdf:resource="http://www.essepuntato.it/2015/07/ido/Price"/>
        <rdfs:comment xml:lang="it">Questa proprietà permette di specificare il prezzo relativo a un certo pezzo come indicato in un ordine o in una fattura.</rdfs:comment>
        <rdfs:comment xml:lang="en">This property allows one to specify the price related to a particular (kind of a) piece as indicated in either in an order or invoice.</rdfs:comment>
        <rdfs:isDefinedBy rdf:resource="http://www.essepuntato.it/2015/07/ido-orders"/>
        <rdfs:label xml:lang="it">ha prezzo per pezzo</rdfs:label>
        <rdfs:label xml:lang="en">has price per piece</rdfs:label>
    </owl:ObjectProperty>
    


    <!-- http://www.essepuntato.it/2015/07/ido/hasTotalValue -->

    <owl:ObjectProperty rdf:about="http://www.essepuntato.it/2015/07/ido/hasTotalValue">
        <owl:inverseOf rdf:resource="http://www.essepuntato.it/2015/07/ido/isTotalValueOf"/>
        <rdfs:domain rdf:resource="http://www.essepuntato.it/2015/07/ido/Order"/>
        <rdfs:range rdf:resource="http://www.essepuntato.it/2015/07/ido/Price"/>
        <rdfs:comment xml:lang="it">La relazione tra un ordine e il valore totale associato.</rdfs:comment>
        <rdfs:comment xml:lang="en">The link between an order and the total price paid by a person for the purchase of that order.</rdfs:comment>
        <rdfs:isDefinedBy rdf:resource="http://www.essepuntato.it/2015/07/ido-orders"/>
        <rdfs:label xml:lang="it">ha valore totale</rdfs:label>
        <rdfs:label xml:lang="en">has total value</rdfs:label>
    </owl:ObjectProperty>
    


    <!-- http://www.essepuntato.it/2015/07/ido/includesPiece -->

    <owl:ObjectProperty rdf:about="http://www.essepuntato.it/2015/07/ido/includesPiece">
        <owl:inverseOf rdf:resource="http://www.essepuntato.it/2015/07/ido/isPieceIncludedIn"/>
        <rdfs:domain rdf:resource="http://www.essepuntato.it/2015/07/ido/Invoice"/>
        <rdfs:range rdf:resource="http://www.essepuntato.it/2015/07/ido/PieceWithPrice"/>
        <rdfs:comment xml:lang="it">Questa proprietà permette di indicare i vari pezzi elencati in una fattura.</rdfs:comment>
        <rdfs:comment xml:lang="en">This property allows one to identify the various pieces included in an invoice.</rdfs:comment>
        <rdfs:isDefinedBy rdf:resource="http://www.essepuntato.it/2015/07/ido-orders"/>
        <rdfs:label xml:lang="it">include pezzo</rdfs:label>
        <rdfs:label xml:lang="en">includes piece</rdfs:label>
    </owl:ObjectProperty>
    


    <!-- http://www.essepuntato.it/2015/07/ido/isPieceIncludedIn -->

    <owl:ObjectProperty rdf:about="http://www.essepuntato.it/2015/07/ido/isPieceIncludedIn">
        <rdfs:comment xml:lang="it">Questa proprietà permette di collegare un particolare pezzo di un capo con la fattura a cui è associato.</rdfs:comment>
        <rdfs:comment xml:lang="en">This property allows one to link a particular piece to the invoice including it.</rdfs:comment>
        <rdfs:isDefinedBy rdf:resource="http://www.essepuntato.it/2015/07/ido-orders"/>
        <rdfs:label xml:lang="en">is peice included in</rdfs:label>
        <rdfs:label xml:lang="it">è incluso come pezzo in</rdfs:label>
    </owl:ObjectProperty>
    


    <!-- http://www.essepuntato.it/2015/07/ido/isTotalValueOf -->

    <owl:ObjectProperty rdf:about="http://www.essepuntato.it/2015/07/ido/isTotalValueOf">
        <rdfs:comment xml:lang="it">La relazione tra il prezzo totale relativo ad un ordine.</rdfs:comment>
        <rdfs:comment xml:lang="en">The link between the total amount of all the items of an order.</rdfs:comment>
        <rdfs:isDefinedBy rdf:resource="http://www.essepuntato.it/2015/07/ido-orders"/>
        <rdfs:label xml:lang="en">is total value of</rdfs:label>
        <rdfs:label xml:lang="it">è valore totale del</rdfs:label>
    </owl:ObjectProperty>
    


    <!-- http://www.essepuntato.it/2015/07/ido/specifiesDistributionPlatform -->

    <owl:ObjectProperty rdf:about="http://www.essepuntato.it/2015/07/ido/specifiesDistributionPlatform">
        <rdfs:comment xml:lang="it">Questa proprietà permette la specificazione di una certa piattaforma di distribuzione associata ad un ordine o ad una fattura.</rdfs:comment>
        <rdfs:comment xml:lang="en">This property allows to specify the particular distribution platform associated to either an order or invoice.</rdfs:comment>
        <rdfs:isDefinedBy rdf:resource="http://www.essepuntato.it/2015/07/ido-orders"/>
        <rdfs:label xml:lang="it">specifica come piattaforma di distribuzione</rdfs:label>
        <rdfs:label xml:lang="en">specifies as distribution platform</rdfs:label>
    </owl:ObjectProperty>
    


    <!-- http://www.essepuntato.it/2015/07/ido/specifiesSalesChannel -->

    <owl:ObjectProperty rdf:about="http://www.essepuntato.it/2015/07/ido/specifiesSalesChannel">
        <rdfs:comment xml:lang="it">Questa proprietà permette la specificazione di una certo canale di vendita associato ad un ordine o ad una fattura.</rdfs:comment>
        <rdfs:comment xml:lang="en">This property allows to specify the particular sales channel associated to either an order or invoice.</rdfs:comment>
        <rdfs:isDefinedBy rdf:resource="http://www.essepuntato.it/2015/07/ido-orders"/>
        <rdfs:label xml:lang="it">specifica come canale di vendita</rdfs:label>
        <rdfs:label xml:lang="en">specifies as sales channel</rdfs:label>
    </owl:ObjectProperty>
    


    <!-- 
    ///////////////////////////////////////////////////////////////////////////////////////
    //
    // Data properties
    //
    ///////////////////////////////////////////////////////////////////////////////////////
     -->

    


    <!-- http://purl.org/dc/terms/identifier -->

    <owl:DatatypeProperty rdf:about="http://purl.org/dc/terms/identifier"/>
    


    <!-- http://purl.org/dc/terms/issued -->

    <owl:DatatypeProperty rdf:about="http://purl.org/dc/terms/issued">
        <rdfs:domain rdf:resource="http://www.w3.org/2002/07/owl#Thing"/>
        <rdfs:range rdf:resource="http://www.w3.org/2000/01/rdf-schema#Literal"/>
        <rdfs:comment xml:lang="en">It allows to specify the issue date of an entity (e.g., an invoice).</rdfs:comment>
        <rdfs:comment xml:lang="it">Permette di specificare la data di immissione di un&apos;entità (per esempio, una fattura).</rdfs:comment>
        <rdfs:isDefinedBy rdf:resource="http://purl.org/dc/terms"/>
        <rdfs:label xml:lang="en">was issued</rdfs:label>
        <rdfs:label xml:lang="it">è stata emessa</rdfs:label>
    </owl:DatatypeProperty>
    


    <!-- http://schema.org/orderDate -->

    <owl:DatatypeProperty rdf:about="http://schema.org/orderDate">
        <rdfs:domain rdf:resource="http://schema.org/Order"/>
        <rdfs:range rdf:resource="http://www.w3.org/2001/XMLSchema#dateTime"/>
        <rdfs:comment xml:lang="it">La proprietà che permette di specificare la data di creazione di un ordine.</rdfs:comment>
        <rdfs:comment xml:lang="en">The property that allows one to specify the order date.</rdfs:comment>
        <rdfs:isDefinedBy rdf:resource="http://schema.org"/>
        <rdfs:label xml:lang="it">ha data di creazione dell&apos;ordine</rdfs:label>
        <rdfs:label xml:lang="en">has order creation date</rdfs:label>
    </owl:DatatypeProperty>
    


    <!-- http://schema.org/orderNumber -->

    <owl:DatatypeProperty rdf:about="http://schema.org/orderNumber">
        <rdfs:isDefinedBy rdf:resource="http://schema.org"/>
    </owl:DatatypeProperty>
    


    <!-- http://schema.org/orderQuantity -->

    <owl:DatatypeProperty rdf:about="http://schema.org/orderQuantity">
        <rdfs:domain rdf:resource="http://schema.org/OrderItem"/>
        <rdfs:range rdf:resource="http://www.w3.org/2001/XMLSchema#decimal"/>
        <rdfs:isDefinedBy rdf:resource="http://schema.org"/>
        <rdfs:isDefinedBy xml:lang="en">It allows one to describe the quantity of a certain article that is requested in an order.</rdfs:isDefinedBy>
        <rdfs:isDefinedBy xml:lang="it">Premettere di indicare la quantità di un certo articolo a seconda di quanto ne sia richiesto in un ordine.</rdfs:isDefinedBy>
        <rdfs:label xml:lang="it">ha quantità ordinata</rdfs:label>
        <rdfs:label xml:lang="en">has order quantity</rdfs:label>
    </owl:DatatypeProperty>
    


    <!-- http://www.essepuntato.it/2015/07/ido/hasOrderIdentifier -->

    <owl:DatatypeProperty rdf:about="http://www.essepuntato.it/2015/07/ido/hasOrderIdentifier">
        <rdfs:subPropertyOf rdf:resource="http://purl.org/dc/terms/identifier"/>
        <rdfs:subPropertyOf rdf:resource="http://schema.org/orderNumber"/>
        <rdfs:domain rdf:resource="http://www.essepuntato.it/2015/07/ido/Order"/>
        <rdfs:comment xml:lang="it">La proprietà che permette di specificare un numero identificativo dell&apos;ordine.</rdfs:comment>
        <rdfs:comment xml:lang="en">The property that allows one to specify the number associated to the order.</rdfs:comment>
        <rdfs:isDefinedBy rdf:resource="http://www.essepuntato.it/2015/07/ido-orders"/>
        <rdfs:label xml:lang="it">ha identificativo d&apos;ordine</rdfs:label>
        <rdfs:label xml:lang="en">has order identifier</rdfs:label>
    </owl:DatatypeProperty>
    


    <!-- 
    ///////////////////////////////////////////////////////////////////////////////////////
    //
    // Classes
    //
    ///////////////////////////////////////////////////////////////////////////////////////
     -->

    


    <!-- http://purl.org/goodrelations/v1#TypeAndQuantityNode -->

    <owl:Class rdf:about="http://purl.org/goodrelations/v1#TypeAndQuantityNode">
        <rdfs:isDefinedBy rdf:resource="http://purl.org/goodrelations/v1"/>
    </owl:Class>
    


    <!-- http://schema.org/Invoice -->

    <owl:Class rdf:about="http://schema.org/Invoice">
        <rdfs:isDefinedBy rdf:resource="http://schema.org"/>
    </owl:Class>
    


    <!-- http://schema.org/Order -->

    <owl:Class rdf:about="http://schema.org/Order">
        <rdfs:isDefinedBy rdf:resource="http://schema.org"/>
    </owl:Class>
    


    <!-- http://schema.org/OrderItem -->

    <owl:Class rdf:about="http://schema.org/OrderItem">
        <rdfs:isDefinedBy rdf:resource="http://schema.org"/>
    </owl:Class>
    


    <!-- http://www.essepuntato.it/2015/07/ido/DistributionPlatform -->

    <owl:Class rdf:about="http://www.essepuntato.it/2015/07/ido/DistributionPlatform">
        <rdfs:comment xml:lang="it">La piattaforma di distribuzione (per esempio B2C o B2B) che può essere usata per distribuire un capo.</rdfs:comment>
        <rdfs:comment xml:lang="en">The distribution platform (e.g., B2C or B2B) that can be used for distributing an item.</rdfs:comment>
        <rdfs:isDefinedBy rdf:resource="http://www.essepuntato.it/2015/07/ido-orders"/>
        <rdfs:label xml:lang="en">distribution platform</rdfs:label>
        <rdfs:label xml:lang="it">piattaforma di distribuzione</rdfs:label>
    </owl:Class>
    


    <!-- http://www.essepuntato.it/2015/07/ido/Invoice -->

    <owl:Class rdf:about="http://www.essepuntato.it/2015/07/ido/Invoice">
        <rdfs:subClassOf rdf:resource="http://schema.org/Invoice"/>
        <rdfs:subClassOf>
            <owl:Restriction>
                <owl:onProperty rdf:resource="http://schema.org/referencesOrder"/>
                <owl:someValuesFrom rdf:resource="http://www.essepuntato.it/2015/07/ido/Order"/>
            </owl:Restriction>
        </rdfs:subClassOf>
        <rdfs:subClassOf>
            <owl:Restriction>
                <owl:onProperty rdf:resource="http://schema.org/totalPaymentDue"/>
                <owl:someValuesFrom rdf:resource="http://www.essepuntato.it/2015/07/ido/Price"/>
            </owl:Restriction>
        </rdfs:subClassOf>
        <rdfs:subClassOf>
            <owl:Restriction>
                <owl:onProperty rdf:resource="http://www.essepuntato.it/2015/07/ido/includesPiece"/>
                <owl:someValuesFrom rdf:resource="http://www.essepuntato.it/2015/07/ido/PieceWithPrice"/>
            </owl:Restriction>
        </rdfs:subClassOf>
        <rdfs:subClassOf>
            <owl:Restriction>
                <owl:onProperty rdf:resource="http://schema.org/referencesOrder"/>
                <owl:allValuesFrom rdf:resource="http://www.essepuntato.it/2015/07/ido/Order"/>
            </owl:Restriction>
        </rdfs:subClassOf>
        <rdfs:subClassOf>
            <owl:Restriction>
                <owl:onProperty rdf:resource="http://schema.org/totalPaymentDue"/>
                <owl:allValuesFrom rdf:resource="http://www.essepuntato.it/2015/07/ido/Price"/>
            </owl:Restriction>
        </rdfs:subClassOf>
        <rdfs:subClassOf>
            <owl:Restriction>
                <owl:onProperty rdf:resource="http://purl.org/dc/terms/identifier"/>
                <owl:cardinality rdf:datatype="http://www.w3.org/2001/XMLSchema#nonNegativeInteger">1</owl:cardinality>
            </owl:Restriction>
        </rdfs:subClassOf>
        <rdfs:subClassOf>
            <owl:Restriction>
                <owl:onProperty rdf:resource="http://purl.org/dc/terms/issued"/>
                <owl:qualifiedCardinality rdf:datatype="http://www.w3.org/2001/XMLSchema#nonNegativeInteger">1</owl:qualifiedCardinality>
                <owl:onDataRange rdf:resource="http://www.w3.org/2001/XMLSchema#dateTime"/>
            </owl:Restriction>
        </rdfs:subClassOf>
        <rdfs:comment xml:lang="en">A list of pieces that have been sent, with a statement of the sum due for these.</rdfs:comment>
        <rdfs:comment xml:lang="it">Una lista di articoli spediti, con informazioni riguardo la spesa totale per il loro acquisto.</rdfs:comment>
        <rdfs:isDefinedBy rdf:resource="http://www.essepuntato.it/2015/07/ido-orders"/>
        <rdfs:label xml:lang="it">fattura</rdfs:label>
        <rdfs:label xml:lang="en">invoice</rdfs:label>
    </owl:Class>
    


    <!-- http://www.essepuntato.it/2015/07/ido/Order -->

    <owl:Class rdf:about="http://www.essepuntato.it/2015/07/ido/Order">
        <rdfs:subClassOf rdf:resource="http://schema.org/Order"/>
        <rdfs:subClassOf>
            <owl:Restriction>
                <owl:onProperty rdf:resource="http://schema.org/orderedItem"/>
                <owl:someValuesFrom rdf:resource="http://www.essepuntato.it/2015/07/ido/StockKeepingUnitAmount"/>
            </owl:Restriction>
        </rdfs:subClassOf>
        <rdfs:subClassOf>
            <owl:Restriction>
                <owl:onProperty rdf:resource="http://www.essepuntato.it/2015/07/ido/hasTotalValue"/>
                <owl:someValuesFrom rdf:resource="http://www.essepuntato.it/2015/07/ido/Price"/>
            </owl:Restriction>
        </rdfs:subClassOf>
        <rdfs:subClassOf>
            <owl:Restriction>
                <owl:onProperty rdf:resource="http://schema.org/orderedItem"/>
                <owl:allValuesFrom rdf:resource="http://www.essepuntato.it/2015/07/ido/StockKeepingUnitAmount"/>
            </owl:Restriction>
        </rdfs:subClassOf>
        <rdfs:subClassOf>
            <owl:Restriction>
                <owl:onProperty rdf:resource="http://schema.org/orderDate"/>
                <owl:qualifiedCardinality rdf:datatype="http://www.w3.org/2001/XMLSchema#nonNegativeInteger">1</owl:qualifiedCardinality>
                <owl:onDataRange rdf:resource="http://www.w3.org/2001/XMLSchema#dateTime"/>
            </owl:Restriction>
        </rdfs:subClassOf>
        <rdfs:subClassOf>
            <owl:Restriction>
                <owl:onProperty rdf:resource="http://www.essepuntato.it/2015/07/ido/hasOrderIdentifier"/>
                <owl:cardinality rdf:datatype="http://www.w3.org/2001/XMLSchema#nonNegativeInteger">1</owl:cardinality>
            </owl:Restriction>
        </rdfs:subClassOf>
        <rdfs:comment xml:lang="it">Questa classe descrive gli ordini di uno o più capi, eseguiti ad una certa ora.</rdfs:comment>
        <rdfs:comment xml:lang="en">This class describes all the orders of one or more articles bought at a certain price and done at a certain time.</rdfs:comment>
        <rdfs:isDefinedBy rdf:resource="http://www.essepuntato.it/2015/07/ido-orders"/>
        <rdfs:label xml:lang="en">order</rdfs:label>
        <rdfs:label xml:lang="it">ordine</rdfs:label>
    </owl:Class>
    


    <!-- http://www.essepuntato.it/2015/07/ido/PieceWithPrice -->

    <owl:Class rdf:about="http://www.essepuntato.it/2015/07/ido/PieceWithPrice">
        <rdfs:subClassOf rdf:resource="http://purl.org/goodrelations/v1#TypeAndQuantityNode"/>
        <rdfs:subClassOf>
            <owl:Restriction>
                <owl:onProperty rdf:resource="http://www.essepuntato.it/2015/07/ido/hasPricePerPiece"/>
                <owl:someValuesFrom rdf:resource="http://www.essepuntato.it/2015/07/ido/Price"/>
            </owl:Restriction>
        </rdfs:subClassOf>
        <rdfs:subClassOf>
            <owl:Restriction>
                <owl:onProperty rdf:resource="http://www.essepuntato.it/2015/07/ido/isPieceIncludedIn"/>
                <owl:someValuesFrom rdf:resource="http://www.essepuntato.it/2015/07/ido/Invoice"/>
            </owl:Restriction>
        </rdfs:subClassOf>
        <rdfs:subClassOf>
            <owl:Restriction>
                <owl:onProperty rdf:resource="http://purl.org/goodrelations/v1#typeOfGood"/>
                <owl:qualifiedCardinality rdf:datatype="http://www.w3.org/2001/XMLSchema#nonNegativeInteger">1</owl:qualifiedCardinality>
                <owl:onClass rdf:resource="http://www.essepuntato.it/2015/07/ido/Piece"/>
            </owl:Restriction>
        </rdfs:subClassOf>
        <rdfs:comment xml:lang="it">Questa classe permette l&apos;identificazione di un pezzo e del relativo prezzo a cui è stato venduto come descritto in una fattura.</rdfs:comment>
        <rdfs:comment xml:lang="en">This class allows the identification of a piece with the related price as recorded in an invoice.</rdfs:comment>
        <rdfs:isDefinedBy rdf:resource="http://www.essepuntato.it/2015/07/ido-orders"/>
        <rdfs:label xml:lang="it">pezzo con prezzo</rdfs:label>
        <rdfs:label xml:lang="en">piece with price</rdfs:label>
    </owl:Class>
    


    <!-- http://www.essepuntato.it/2015/07/ido/SalesChannel -->

    <owl:Class rdf:about="http://www.essepuntato.it/2015/07/ido/SalesChannel">
        <rdfs:comment xml:lang="it">Il canale di vendita (ad esempio, e-commerce) che può essere usato per vendere/comprare un capo.</rdfs:comment>
        <rdfs:comment xml:lang="en">The sales channel (e.g., e-commerce) that can be used for buying/selling an item.</rdfs:comment>
        <rdfs:isDefinedBy rdf:resource="http://www.essepuntato.it/2015/07/ido-orders"/>
        <rdfs:label xml:lang="it">canale di vendita</rdfs:label>
        <rdfs:label xml:lang="en">sales channel</rdfs:label>
    </owl:Class>
    


    <!-- http://www.essepuntato.it/2015/07/ido/StockKeepingUnitAmount -->

    <owl:Class rdf:about="http://www.essepuntato.it/2015/07/ido/StockKeepingUnitAmount">
        <rdfs:subClassOf rdf:resource="http://purl.org/goodrelations/v1#TypeAndQuantityNode"/>
        <rdfs:subClassOf rdf:resource="http://schema.org/OrderItem"/>
        <rdfs:subClassOf>
            <owl:Restriction>
                <owl:onProperty rdf:resource="http://www.essepuntato.it/2015/07/ido/hasPricePerPiece"/>
                <owl:someValuesFrom rdf:resource="http://www.essepuntato.it/2015/07/ido/Price"/>
            </owl:Restriction>
        </rdfs:subClassOf>
        <rdfs:subClassOf>
            <owl:Restriction>
                <owl:onProperty>
                    <rdf:Description>
                        <owl:inverseOf rdf:resource="http://schema.org/orderedItem"/>
                    </rdf:Description>
                </owl:onProperty>
                <owl:someValuesFrom rdf:resource="http://www.essepuntato.it/2015/07/ido/Order"/>
            </owl:Restriction>
        </rdfs:subClassOf>
        <rdfs:subClassOf>
            <owl:Restriction>
                <owl:onProperty rdf:resource="http://purl.org/goodrelations/v1#typeOfGood"/>
                <owl:qualifiedCardinality rdf:datatype="http://www.w3.org/2001/XMLSchema#nonNegativeInteger">1</owl:qualifiedCardinality>
                <owl:onClass rdf:resource="http://www.essepuntato.it/2015/07/ido/StockKeepingUnit"/>
            </owl:Restriction>
        </rdfs:subClassOf>
        <rdfs:subClassOf>
            <owl:Restriction>
                <owl:onProperty rdf:resource="http://schema.org/orderQuantity"/>
                <owl:qualifiedCardinality rdf:datatype="http://www.w3.org/2001/XMLSchema#nonNegativeInteger">1</owl:qualifiedCardinality>
                <owl:onDataRange rdf:resource="http://www.w3.org/2001/XMLSchema#positiveInteger"/>
            </owl:Restriction>
        </rdfs:subClassOf>
        <rdfs:comment xml:lang="it">Questa classe describe la quantità richiesta di un certo articolo gestito in magazzino come indicato in un ordine.</rdfs:comment>
        <rdfs:comment xml:lang="en">This class describes the requested amount of a particular stock keeping unit as recorded in an order.</rdfs:comment>
        <rdfs:isDefinedBy rdf:resource="http://www.essepuntato.it/2015/07/ido-orders"/>
        <rdfs:label xml:lang="it">quantità dell&apos;articolo gestito in magazzino</rdfs:label>
        <rdfs:label xml:lang="en">stock keeping unit amount</rdfs:label>
    </owl:Class>
    


    <!-- http://www.w3.org/2002/07/owl#Thing -->

    <owl:Class rdf:about="http://www.w3.org/2002/07/owl#Thing"/>
    


    <!-- 
    ///////////////////////////////////////////////////////////////////////////////////////
    //
    // Individuals
    //
    ///////////////////////////////////////////////////////////////////////////////////////
     -->

    


    <!-- http://www.essepuntato.it/2015/07/ido/b2b -->

    <owl:NamedIndividual rdf:about="http://www.essepuntato.it/2015/07/ido/b2b">
        <rdf:type rdf:resource="http://www.essepuntato.it/2015/07/ido/DistributionPlatform"/>
        <rdfs:comment xml:lang="en">Business-to-business (B2B) refers to distribution platform where one business makes a commercial transaction with another.</rdfs:comment>
        <rdfs:comment xml:lang="it">La distribuzione via commercio interaziendale si applica quando un&apos;azienda effettua una transazione commerciale con un&apos;altra.</rdfs:comment>
        <rdfs:isDefinedBy rdf:resource="http://www.essepuntato.it/2015/07/ido-orders"/>
        <rdfs:label xml:lang="en">business to business</rdfs:label>
        <rdfs:label xml:lang="it">commercio interaziendale</rdfs:label>
    </owl:NamedIndividual>
    


    <!-- http://www.essepuntato.it/2015/07/ido/b2c -->

    <owl:NamedIndividual rdf:about="http://www.essepuntato.it/2015/07/ido/b2c">
        <rdf:type rdf:resource="http://www.essepuntato.it/2015/07/ido/DistributionPlatform"/>
        <rdfs:comment xml:lang="en">Business-to-consumer (B2C) refers to distribution platform where one business makes a commercial transaction with a consumer.</rdfs:comment>
        <rdfs:comment xml:lang="it">La distribuzione via vendita al dettaglio si applica quando un&apos;azienda effettua una transazione commerciale con un consumatore finale.</rdfs:comment>
        <rdfs:isDefinedBy rdf:resource="http://www.essepuntato.it/2015/07/ido-orders"/>
        <rdfs:label xml:lang="en">business to consumer</rdfs:label>
        <rdfs:label xml:lang="it">vendita al dettaglio</rdfs:label>
    </owl:NamedIndividual>
    


    <!-- http://www.essepuntato.it/2015/07/ido/e-commerce -->

    <owl:NamedIndividual rdf:about="http://www.essepuntato.it/2015/07/ido/e-commerce">
        <rdf:type rdf:resource="http://www.essepuntato.it/2015/07/ido/SalesChannel"/>
        <rdfs:comment xml:lang="en">Electronic commerce, commonly written as e-commerce, is the a sales channel for products or services using computer networks, such as the Internet.</rdfs:comment>
        <rdfs:comment xml:lang="it">Il commercio elettronico è un canale per la vendita dei prodotti o servizi che fa uso di reti di calcolatori, ad esempio Internet.</rdfs:comment>
        <rdfs:isDefinedBy rdf:resource="http://www.essepuntato.it/2015/07/ido-orders"/>
        <rdfs:label xml:lang="it">commercio elettronico</rdfs:label>
        <rdfs:label xml:lang="en">electronic commerce</rdfs:label>
    </owl:NamedIndividual>
    


    <!-- http://www.essepuntato.it/2015/07/ido/front-desk -->

    <owl:NamedIndividual rdf:about="http://www.essepuntato.it/2015/07/ido/front-desk">
        <rdf:type rdf:resource="http://www.essepuntato.it/2015/07/ido/SalesChannel"/>
        <rdfs:comment xml:lang="en">Front desk commerce is the a sales channel for products or services using direct and physical interaction between the seller and the buyer.</rdfs:comment>
        <rdfs:comment xml:lang="it">Il commercio diretto è un canale di vendita per prodotti e servizi che usa l&apos;interazione diretta e fisica tra un venditore e un compratore.</rdfs:comment>
        <rdfs:isDefinedBy rdf:resource="http://www.essepuntato.it/2015/07/ido-orders"/>
        <rdfs:label xml:lang="it">commercio diretto</rdfs:label>
        <rdfs:label xml:lang="en">front desk commerce</rdfs:label>
    </owl:NamedIndividual>
    <rdf:Description>
        <owl:cardinality rdf:datatype="http://www.w3.org/2001/XMLSchema#nonNegativeInteger">1</owl:cardinality>
    </rdf:Description>
</rdf:RDF>



<!-- Generated by the OWL API (version 4.2.1.20160306-0033) https://github.com/owlcs/owlapi -->

